PFourInARow.v
@@ -1,0 +1,1086 @@
+
+From Stdlib Require Import ssreflect ZArith Ascii List String PrimInt63.
+From Stdlib Require Import PArray.
+From mathcomp Require Import ssrnat ssrbool div fintype eqtype seq.
+From Stdlib Require Import Lia.
+Require Import ssr_int.
+Require Import FourInARow.
+
+Import PrimInt63Notations.
+Import Uint63Axioms.
+Import Uint63.
+
+Open Scope uint63_scope.
+
+Lemma init_matrix_length1 (A : Type) n nn a (v : A) m : 
+  nn <=? length a -> (Z.of_nat n <= φ nn)%Z ->  
+  length (init_matrix n nn a v m) = length a.
+Proof.
+elim: n nn a  => //= n IH nn a nLa nLm.
+have /lebP tnLa := nLa.
+have nnB := to_Z_bounded nn.
+have nn1E : to_Z (nn - 1) = (to_Z nn - 1)%Z.
+  by rewrite sub_spec ?to_Z_1 Z.mod_small; lia.
+by rewrite IH ?length_set //; (try apply/lebP); lia.
+Qed.
+
+Lemma init_matrix_length2 (A : Type) n nn a (v : A) m i : 
+    m <=? max_length ->
+    (Z.of_nat n <= to_Z nn)%Z -> nn <=? length a ->
+    (to_Z i + Z.of_nat n < wB)%Z ->
+    if (nn <=? i + of_nat n) && (i <? nn) then
+       length (init_matrix n nn a v m).[i] = m
+    else length (init_matrix n nn a v m).[i] = length (a.[i]).
+Proof.
+move=> mLm.
+elim: n nn a => [|n IH] nn a Ha.
+  rewrite Z.add_0_r => Hn.
+  case: lebP => /=; rewrite add_spec //. 
+  rewrite to_Z_0 Z.add_0_r Z.mod_small; last by apply: to_Z_bounded.
+  by case: ltbP => //; lia.
+move=> Hn H1.
+have nnB := to_Z_bounded nn.
+have nLw : (Z.of_nat n < wB)%Z by lia.
+have nB := to_Z_bounded (of_nat n).
+have znnsP : (0 < to_Z nn)%Z by lia.
+have nn1E : to_Z (nn - 1) = (to_Z nn - 1)%Z.
+  by  rewrite sub_spec ?to_Z_1 Z.mod_small; lia.
+have F : (Z.of_nat n <= to_Z (nn - 1))%Z by lia.
+have F' : nn - 1 <=? length a.[nn - 1<-make m v].
+  apply/lebP; rewrite nn1E length_set.
+  by have /lebP := Hn; lia.
+have iB := to_Z_bounded i.
+have n1B := to_Z_bounded (of_nat n.+1).
+have F1 : (to_Z i + Z.of_nat n < wB)%Z by lia.
+have F2 : to_Z (of_nat n) = (Z.of_nat n)%Z.
+  by rewrite of_Z_spec Z.mod_small; lia.
+have F3 : to_Z (of_nat n.+1) = (Z.of_nat n + 1)%Z.
+  by rewrite of_Z_spec Z.mod_small; lia.
+have F4 : φ (i + of_nat n.+1) =  (φ i + Z.of_nat n + 1)%Z.
+  by rewrite add_spec Z.mod_small; lia.
+have F5 : φ (i + of_nat n) =  (φ i + Z.of_nat n)%Z.
+  by rewrite add_spec Z.mod_small; lia.
+have n1E : to_Z (nn - 1) = ((to_Z nn) - 1)%Z.
+  by rewrite sub_spec ?to_Z_1 Z.mod_small; lia.
+case: lebP => //=; last first.
+  rewrite F4.
+  move/Z.nle_gt => H3.
+  have := IH (nn - 1) a.[nn - 1<-make m v] F F'.
+  rewrite ifN; last first.
+    by case: lebP; rewrite ?n1E  F5 //; lia.
+  move=> ->; try lia.
+  rewrite get_set_other // => HH.
+  by move: H3; rewrite -HH n1E; lia.
+rewrite F4 => H3.
+case: ltbP => [H4|/Z.nlt_ge H4]; last first.
+  have := IH (nn - 1) a.[nn - 1<-make m v] F F'.
+  rewrite ifN //.
+    rewrite get_set_other //.
+    apply; lia.
+    by move=> HH; move: H4; rewrite -HH; lia.
+  rewrite andbC negb_and; case: ltbP => //.
+  by rewrite n1E; lia.
+have := IH (nn - 1) a.[nn - 1<-make m v] F F'.
+case: lebP; rewrite F5 n1E; try lia.
+case: ltbP; rewrite n1E //= => V1 V2 -> //; try lia.
+suff H : nn - 1 = i.
+  rewrite H get_set_same.
+    by rewrite length_make // ?mLm.
+  case ltbP; try lia.
+  have /lebP := Hn; lia.
+apply: to_Z_inj.
+by rewrite n1E; lia.
+Qed.
+
+Lemma init_matrix_get (A : Type) n nn a (v : A) m i j : 
+    m <=? max_length ->
+    j <? m ->
+    (Z.of_nat n <= to_Z nn)%Z -> nn  <=? length a ->
+    (to_Z i + Z.of_nat n < wB)%Z ->
+    if (nn <=? i + of_nat n) && (i <? nn) then
+      (init_matrix n nn a v m).[i].[j] = v
+    else (init_matrix n nn a v m).[i].[j] = a.[i].[j].
+Proof.
+move=> mLm jLn.
+elim: n nn a => [|n IH] nn a Ha.
+  rewrite Z.add_0_r => Hn.
+  case: lebP => //=; rewrite add_spec //. 
+  rewrite to_Z_0 Z.add_0_r Z.mod_small; last by apply: to_Z_bounded.
+  by case: ltbP => //; lia.
+move=> Hn H1.
+have nnB := to_Z_bounded nn.
+have nLw : (Z.of_nat n < wB)%Z by lia.
+have nB := to_Z_bounded (of_nat n).
+have znnsP : (0 < to_Z nn)%Z by lia.
+have nn1E : to_Z (nn - 1) = (to_Z nn - 1)%Z.
+  by  rewrite sub_spec ?to_Z_1 Z.mod_small; lia.
+have F : (Z.of_nat n <= to_Z (nn - 1))%Z by lia.
+have F' : nn - 1 <=? length a.[nn - 1<-make m v].
+  apply/lebP; rewrite nn1E length_set.
+  by have /lebP := Hn; lia.
+have iB := to_Z_bounded i.
+have n1B := to_Z_bounded (of_nat n.+1).
+have F1 : (to_Z i + Z.of_nat n < wB)%Z by lia.
+have F2 : to_Z (of_nat n) = (Z.of_nat n)%Z.
+  by rewrite of_Z_spec Z.mod_small; lia.
+have F3 : to_Z (of_nat n.+1) = (Z.of_nat n + 1)%Z.
+  by rewrite of_Z_spec Z.mod_small; lia.
+have F4 : φ (i + of_nat n.+1) =  (φ i + Z.of_nat n + 1)%Z.
+  by rewrite add_spec Z.mod_small; lia.
+have F5 : φ (i + of_nat n) =  (φ i + Z.of_nat n)%Z.
+  by rewrite add_spec Z.mod_small; lia.
+have n1E : to_Z (nn - 1) = ((to_Z nn) - 1)%Z.
+  by rewrite sub_spec ?to_Z_1 Z.mod_small; lia.
+case: lebP => //=; last first.
+  rewrite F4.
+  move/Z.nle_gt => H3.
+  have := IH (nn - 1) a.[nn - 1<-make m v] F F'.
+  rewrite ifN; last first.
+    by case: lebP; rewrite ?n1E  F5 //; lia.
+  move=> ->; try lia.
+  rewrite get_set_other // => HH.
+  by move: H3; rewrite -HH n1E; lia.
+rewrite F4 => H3.
+case: ltbP => [H4|/Z.nlt_ge H4]; last first.
+  have := IH (nn - 1) a.[nn - 1<-make m v] F F'.
+  rewrite ifN //.
+    rewrite get_set_other //.
+    apply; lia.
+    by move=> HH; move: H4; rewrite -HH; lia.
+  rewrite andbC negb_and; case: ltbP => //.
+  by rewrite n1E; lia.
+have := IH (nn - 1) a.[nn - 1<-make m v] F F'.
+case: lebP; rewrite F5 n1E; try lia.
+case: ltbP; rewrite n1E //= => V1 V2 -> //; try lia.
+suff H : nn - 1 = i.
+  rewrite H get_set_same.
+    by rewrite get_make //.
+  case ltbP; try lia.
+  have /lebP := Hn; lia.
+apply: to_Z_inj.
+by rewrite n1E; lia.
+Qed.
+
+Lemma make_matrix_length1 (A : Type) n m (v : A) :
+   n <=? max_length -> length (make_matrix n m v) = n.
+Proof.
+move=> nLl.
+have nB := to_Z_bounded n.
+rewrite init_matrix_length1 //.
+rewrite length_make // nLl //.
+rewrite length_make nLl; apply/lebP; lia.
+by rewrite Z2Nat.id; lia.
+Qed.
+
+Lemma make_matrix_length2 (A : Type) n m  (v : A) i : 
+    n <=? max_length -> 
+    m <=? max_length ->
+    i <? n -> length (make_matrix n m v).[i] = m.
+Proof.
+move=> nLl mLl iLn.
+rewrite /make_matrix /=.
+have nB := to_Z_bounded n.
+have F1 : (Z.of_nat (to_nat n) <= φ (n))%Z by rewrite Z2Nat.id; lia.
+have F2 : n ≤? length (make n (make 0 v)).
+  by apply/lebP; rewrite length_make nLl; lia.
+have F3 : (φ (i) + Z.of_nat (to_nat n) < wB)%Z.
+  rewrite Z2Nat.id; try lia.
+  have /lebP := nLl; have/ltbP := iLn.
+  set u := to_Z max_length; compute in u; rewrite /u.
+  set w := wB; compute in w; rewrite /w.
+  lia.
+have := init_matrix_length2 _ (to_nat n) n (make n (make 0 v)) 
+               v m i mLl F1 F2 F3.
+have iB := to_Z_bounded i.
+rewrite iLn andbT ifT //.
+by apply/lebP; rewrite add_spec of_Z_spec !Z.mod_small; try lia.
+Qed.
+
+Lemma make_matrix_get (A : Type) n m  (v : A) i j : 
+    n <=? max_length -> m <=? max_length ->
+    i <? n -> j <? m ->
+    (make_matrix n m v).[i].[j] = v.
+Proof.
+move=> nLl mLl iLn jLm.
+rewrite /make_matrix /=.
+have nB := to_Z_bounded n.
+have F1 : (Z.of_nat (to_nat n) <= φ (n))%Z by rewrite Z2Nat.id; lia.
+have F2 : n ≤? length (make n (make 0 v)).
+  by apply/lebP; rewrite length_make nLl; lia.
+have F3 : (φ (i) + Z.of_nat (to_nat n) < wB)%Z.
+  rewrite Z2Nat.id; try lia.
+  have /lebP := nLl; have/ltbP := iLn.
+  set u := to_Z max_length; compute in u; rewrite /u.
+  set w := wB; compute in w; rewrite /w.
+  lia.
+have := init_matrix_get _ (to_nat n) n (make n (make 0 v)) 
+               v m i j mLl jLm F1 F2 F3.
+have iB := to_Z_bounded i.
+rewrite iLn andbT ifT //.
+by apply/lebP; rewrite add_spec of_Z_spec !Z.mod_small; lia.
+Qed.
+
+Lemma bit_decr i j : j <? digits -> bit (decr (one << j)) i = (i <? j).
+Proof.
+case: ltbP => // => jLs.
+have iB := to_Z_bounded i.
+have jB := to_Z_bounded j.
+have Fi : (1 <= 2 ^ to_Z i)%Z by apply: (Z.pow_le_mono_r _ 0); lia.
+have Fn : (1 <= 2 ^ to_Z j)%Z by apply: (Z.pow_le_mono_r _ 0); lia. 
+rewrite bitE.
+have FE : IntDef.Z.of_nat size = φ (digits) by [].
+rewrite  /decr sub_spec ?to_Z_1 Z.mod_small; last first.
+  rewrite lsl_spec Z.mul_1_l Z.mod_small; split; try lia.
+    suff : (2 ^ φ (j) <= wB)%Z by lia.
+    by apply: Z.pow_le_mono_r; rewrite ?FE; lia.
+  by apply: Z.pow_lt_mono_r; rewrite ?FE; lia.
+rewrite lsl_spec Z.mod_small Z.mul_1_l; last first.
+  split; try lia.
+  by apply: Z.pow_lt_mono_r; rewrite ?FE; lia.
+rewrite Z.testbit_eqb; last by lia.
+case: ltbP => [iLn|/Z.nlt_ge nLi]; last first.
+  rewrite Z.div_small //; split; try lia.
+  suff: (2 ^ to_Z j <= 2 ^ to_Z i)%Z by lia.
+  by apply: Z.pow_le_mono_r; rewrite ?FE; lia.
+have -> : (2 ^ φ j - 1 = 
+           (2 ^ (φ j - φ i) - 1) * 2 ^ φ i + (2 ^ (φ i) - 1))%Z.
+  rewrite Z.mul_add_distr_r.
+  rewrite -Zpower_exp; try lia.
+  have -> : (φ j - φ (i) + φ (i)  = φ j)%Z by lia.
+  lia.
+rewrite Z.div_add_l; try lia.
+rewrite Z.div_small ?Z.add_0_r; try lia.
+rewrite Zminus_mod.
+have -> : (φ j - φ (i) = (1 + (φ j - φ (i) -1)))%Z by lia.
+rewrite Zpower_exp; try lia.
+by rewrite Z.mul_mod.
+Qed.
+
+Lemma all_set_spec i : bit all_set i = (i <? number_of_cells).
+Proof. by apply: bit_decr. Qed.
+
+Lemma first_colum_spec i : bit first_column i = (i <? height).
+Proof. by apply: bit_decr. Qed.
+
+Lemma full_first_colum_spec i : bit full_first_column i = (i <? horizontal).
+Proof. by apply: bit_decr. Qed.
+
+Lemma bottom_spec i : 
+  bit bottom i = ((i mod horizontal =? 0) && (i <? width * horizontal)).
+Proof.
+have F1 : (1 < 2 ^ φ (horizontal))%Z by apply: (Z.pow_lt_mono_r _ 0).
+have F2 : (1 < 2 ^ φ (number_of_cells))%Z by apply: (Z.pow_lt_mono_r _ 0).
+have F3 : (2 ^ φ (horizontal) < wB)%Z by apply: Z.pow_lt_mono_r.
+have F4 : (2 ^ φ (number_of_cells) < wB)%Z by apply: Z.pow_lt_mono_r.
+have F5 := to_Z_bounded i.
+have F6 : (0 <= φ (horizontal))%Z by compute.
+have F7 : (2 <= 2 ^ φ (horizontal))%Z by compute.
+have F8 : (0 <= φ (width))%Z by compute.
+have F9 k l : 
+  (1 <= l -> 0 <= k -> 
+    (2 ^ ((1 + k) * l) - 1) / (2 ^ l - 1)  =
+       (2 ^ (k * l) + (2 ^ (k * l) - 1) / (2 ^ l - 1)))%Z.
+  move=> lP kP.
+  have l2P : (2 <= 2 ^ l)%Z by apply: (Z.pow_le_mono_r 2 1); lia.
+  replace (2 ^ ((1 + k) * l) - 1)%Z with
+    (2 ^ (k * l) * (2 ^ l - 1) + (2 ^ (k * l) - 1))%Z; last first.
+    by rewrite Z.mul_add_distr_r Z.mul_1_l Zpower_exp; lia.
+  by rewrite Z_div_plus_full_l //; lia.
+have F10 k l : 
+  (1 <= l -> 0 <= k -> 
+    (2 ^ (k * l) - 1) / (2 ^ l - 1) < 2 ^ (k * l))%Z.
+  move=> lP.
+  have l2P : (2 <= 2 ^ l)%Z by apply: (Z.pow_le_mono_r 2 1); lia.
+  move: k.
+  apply: natlike_ind; first by compute.
+  move=> k kP IH.
+  rewrite -Z.add_1_l F9 //.
+  rewrite Z.mul_add_distr_r Z.mul_1_l Zpower_exp; try lia.
+  suff : (2 ^ (k * l) * 2 <= 2 ^ (k * l) * 2 ^ l)%Z by lia.
+  by apply: Zmult_le_compat_l; lia.
+rewrite bitE.
+rewrite div_spec !sub_spec to_Z_1 !lsl_spec !Z.mul_1_l !Z.mod_small; 
+  try split; try lia.
+rewrite Z.testbit_eqb; try lia.
+rewrite mul_spec [((_ * _) mod _)%Z]Z.mod_small; last by compute.
+case: ltbP => [iLw|/Z.nlt_ge wLi]; last first.
+  rewrite mul_spec [((_ * _) mod _)%Z]Z.mod_small in wLi; last by compute.
+  rewrite andbF Z.div_small; first by [].
+  split; first by compute.
+  apply: Z.lt_le_trans; last by apply: Z.pow_le_mono_r wLi.
+  by apply: F10.
+rewrite andbT.
+rewrite mul_spec Z.mod_small in iLw; last by split; try lia; compute.
+have -> : (i mod horizontal =? 0) = ((to_Z i mod (to_Z horizontal)) =? 0)%Z.
+  case: Uint63.eqbP.
+    by rewrite mod_spec => ->.
+  by rewrite mod_spec; case: (_ mod _)%Z.
+rewrite {1}(Z.div_mod (to_Z i) (to_Z horizontal)); try lia.
+rewrite Zpower_exp; last 2 first.
+- apply: Z.le_ge.
+  apply: Z.mul_nonneg_nonneg; try lia.
+  by apply: Z.div_pos; lia.
+- apply: Z.le_ge.
+  by have := (Z_mod_lt (to_Z i) (to_Z horizontal)); try lia.
+rewrite -Z.div_div; last 2 first.
+- suff : (0 < 2 ^ (φ (horizontal) * (φ (i) / φ (horizontal))))%Z by lia.
+  apply: Z.pow_pos_nonneg; try lia.
+  apply: Z.mul_nonneg_nonneg; try lia.
+  by apply: Z.div_pos; lia.
+- apply: Z.pow_pos_nonneg; try lia.
+  by have := (Z_mod_lt (to_Z i) (to_Z horizontal)); try lia.
+set q := (_ / to_Z _)%Z; set m := (_ mod to_Z _)%Z.
+have qP : (0 <= q)%Z by apply: Z_div_pos; lia.
+have mP : (0 <= m < to_Z horizontal)%Z by  apply: Z.mod_bound_pos; lia.
+have m2P : (1 <= 2 ^ m)%Z by apply: (Z.pow_le_mono_r 2 0); lia.
+have wL : (q < to_Z width)%Z by apply: Z.div_lt_upper_bound; lia.
+replace (to_Z width) with ((to_Z width - q - 1) + 1 + q)%Z by lia.
+have : (0 <=  φ (width) - q - 1)%Z by lia.
+elim/natlike_ind : (_ - _)%Z; last by lia.
+  set u := φ (horizontal).
+  rewrite Z.add_0_l F9 //.
+  have uqP : (1 <= 2 ^ (u * q))%Z by apply: (Z.pow_le_mono_r 2 0); lia.
+  replace (q * u)%Z with (u * q)%Z by lia.
+  rewrite -{1}[(2  ^ (u * q))%Z]Z.mul_1_l Z.div_add_l; last by lia.
+  rewrite [(_ / 2 ^ (_ * _))%Z]Z.div_small.
+    case: (Z.eqb_spec m 0) => [->|mPP].
+      by compute.
+    have l2P : (2 <= 2 ^ m)%Z by apply: (Z.pow_le_mono_r 2 1); lia.
+    by rewrite Z.div_small //; lia.
+  split.
+    apply: Z.div_pos; try lia.
+    have uP : (1 <= u)%Z by compute.
+    suff : (2 <= 2 ^ u)%Z by lia.
+    by apply: (Z.pow_le_mono_r 2 1); lia.
+  replace (u * q)%Z with (q * u)%Z by lia.
+  by apply: F10; lia.
+move=> k kP IH _.
+have HH : (1 <= 2 ^ (φ (horizontal) * q))%Z 
+  by apply: (Z.pow_le_mono_r 2 0); try lia.
+replace (Z.succ k + 1 + q)%Z with (1 + (k + 1 + q))%Z by lia.
+rewrite F9; try lia.
+rewrite {1}Z.mul_add_distr_r; try lia.
+rewrite Zpower_exp; try lia.
+replace (q * φ (horizontal))%Z with (φ (horizontal) * q)%Z by lia.
+rewrite Z.div_add_l; try lia.
+replace ((k + 1) * φ (horizontal))%Z with 
+          ((k * φ (horizontal)) + (φ (horizontal) - m) + m)%Z by lia.
+rewrite Zpower_exp; try lia.
+rewrite Z.div_add_l; try lia.
+rewrite Z.add_mod; try lia.
+suff : (2 | 2 ^ (k * φ (horizontal) + (φ (horizontal) - m)))%Z.
+  rewrite -Z.mod_divide; try lia.
+  move=>->.
+  by rewrite Z.add_0_l Z.mod_mod; lia.
+exists (2 ^ (k * φ (horizontal) + (φ (horizontal) - m) - 1))%Z.
+rewrite -(Zpower_exp _ _ 1); try lia.
+congr (2 ^ _)%Z.
+lia.
+Qed.
+
+Lemma top_spec i : 
+  bit top i = ((i mod horizontal =? height) && (i <? width * horizontal)).
+Proof.
+have iP := to_Z_bounded i.
+rewrite bit_lsl bottom_spec.
+case: lebP=> //.
+  rewrite orbT.
+  move=> H1; case: ltbP => //.
+    have : (to_Z  (width * horizontal) < φ (digits))%Z by compute.
+    by lia.
+  by rewrite andbF.
+have H1 : (to_Z height < to_Z horizontal)%Z by compute.  
+rewrite orbF => /Z.nle_gt H2.
+case: ltbP=> //.
+  move=> H3; case: Uint63.eqbP => //.
+  by rewrite mod_spec Z.mod_small; lia.
+move/Z.nlt_ge => H4.
+have hP : (0 <= to_Z height)%Z by compute.
+case: eqbP  => //; 
+    rewrite mod_spec to_Z_0 sub_spec (Z.mod_small _ wB); try lia; last first.
+  case: Uint63.eqbP => //.
+  rewrite mod_spec.
+  rewrite Zminus_mod => ->.
+  rewrite Zminus_mod Zmod_mod -Zminus_mod.
+  by rewrite Z.sub_diag Z.mod_0_l; lia.
+move=> H5.
+case: eqbP  => //; last first.
+  case.
+  rewrite mod_spec; try by lia.
+  replace (to_Z i) with ((to_Z i - to_Z height) + to_Z height)%Z by lia.
+  rewrite Z.add_mod; try lia.
+  rewrite H5 Z.add_0_l Z.mod_mod; try lia.
+  by rewrite Z.mod_small; lia.
+do 2 case: ltbP; try lia; last first.
+  by rewrite sub_spec Z.mod_small; lia.
+rewrite mul_spec [((_ * _) mod _)%Z]Z.mod_small; last by compute.
+move=> /Z.nlt_ge => H6.
+rewrite sub_spec Z.mod_small; try lia.
+move=> H7.
+    rewrite mod_spec.
+replace (φ  i) with (φ (width) * φ (horizontal) +
+                        (φ i - (φ (width) * φ (horizontal))))%Z by lia.
+rewrite Z.add_mod; try lia.
+rewrite Z.mul_mod; try lia.
+rewrite Z.mod_same; try lia.
+rewrite Z.mod_0_l; try lia.
+rewrite Z.add_0_l Z.mod_mod; try lia.
+by rewrite Z.mod_small; lia.
+Qed.
+
+Lemma bit_mhash i : bit mhash i = (i <? lhash).
+Proof. by apply: bit_decr. Qed.
+
+Lemma make_hash_length1 (u : unit) : length (make_hash u) = nhash.
+Proof. by apply: make_matrix_length1. Qed.
+
+Lemma make_hash_length2 (u : unit) i : 
+   i <? nhash -> length (make_hash u).[i] = (2 * (hprime/nhash) + 1).
+Proof. by move=> iLn; apply: make_matrix_length2. Qed.
+
+Lemma make_hash_get (u : unit) i j : 
+    i <? nhash -> j <? 2 * (hprime/nhash) + 1 ->
+    (make_hash u).[i].[j] = 0.
+Proof. by move=> nLi mLj; apply: make_matrix_get. Qed.
+
+Lemma bit_logand2_aux s dir i : 
+  dir <=? digits ->
+  bit (s land s >> dir land (s land s >> dir) >> (2 * dir)) i =
+                   [&&
+                       bit s i, bit s (i + dir),
+                       bit s (i + 2 * dir) & bit s (i + 3 * dir)].
+Proof.
+case: lebP => // dirP1 _.
+have iP := to_Z_bounded i.
+have dirP := to_Z_bounded dir.
+have dir2P := to_Z_bounded (2 * dir).
+have dir3P := to_Z_bounded (3 * dir).
+have Fp : (φ (digits) < wB)%Z.
+  by rewrite /wB /= /IntDef.Z.pow_pos /= /digits /to_Z /=; lia.
+have F2p : (2 * φ (digits) < wB)%Z.
+  by rewrite /wB /= /IntDef.Z.pow_pos /= /digits /to_Z /=; lia.
+rewrite !(land_spec, bit_lsr).
+case: (Z.ltb_spec (φ (i)) (φ (digits))) => Hphi; last first.
+  by rewrite bit_M => //; case: lebP; lia.
+case: bit => //=. 
+(case: lebP; rewrite add_spec) => [_|]; last first.
+  by rewrite Z.mod_small; try lia.
+rewrite add_comm.
+case: (Z.ltb_spec (φ (i) + φ (dir)) (φ (digits))) => Hphi1; last first.
+  rewrite bit_M => //; case: lebP; try lia.
+  rewrite add_spec Z.mod_small; try lia.
+case: bit => //=.
+rewrite add_comm. 
+case: (Z.ltb_spec (φ (i) + 2 * φ (dir)) (φ (digits))) => Hphi2; last first.
+  rewrite bit_M => //; case: lebP; try lia.
+  rewrite add_spec Z.mod_small; try lia.
+    by rewrite mul_spec -[to_Z 2]/2%Z Z.mod_small; lia.
+  by rewrite mul_spec -[to_Z 2]/2%Z Z.mod_small; lia.
+case: lebP;  rewrite !(add_spec, mul_spec) -[to_Z 2]/2%Z !Z.mod_small; try lia.
+move=> HF.
+case bit => //=.
+have -> : dir + (i + 2 * dir) = i + 3 * dir.
+  apply: to_Z_inj.
+  by rewrite !(add_spec, mul_spec) -[to_Z 2]/2%Z -[to_Z 3]/3%Z !Z.mod_small; lia.
+case: (Z.ltb_spec (φ (i) + 3 * φ (dir)) (φ (digits))) => Hphi3; last first.
+  rewrite bit_M => //; case: lebP; try lia.
+  by rewrite !(add_spec, mul_spec) -[to_Z 3]/3%Z !Z.mod_small; lia.
+case: lebP => //.
+by rewrite !(add_spec, mul_spec) -[to_Z 2]/2%Z -[to_Z 3]/3%Z !Z.mod_small; lia.
+Qed.
+
+Lemma bit_logand2 s dir dir2 : 
+  dir <=? digits -> dir2 = 2 * dir ->
+  logand2 s dir dir2 = [forall i, 
+                       ~~ [&& bit s i, bit s (i + dir),
+                              bit s (i + 2 * dir) & bit s (i + 3 * dir)]].
+Proof.
+move=> Hd Hd2.
+rewrite /logand2 is_zeroP /= Hd2.
+apply/forallP/forallP => /= H i.
+  by have := H i; rewrite bit_logand2_aux.
+by rewrite bit_logand2_aux; have := H i.
+Qed.
+
+Lemma bit_is_won s  : 
+  is_won s  = [exists i,
+                [exists dir,
+                   [&&
+                      dir \in [:: horizontal; vertical; up_left; up_right],
+                      bit s i, bit s (i + dir),
+                          bit s (i + 2 * dir) & bit s (i + 3 * dir)]]].
+Proof.
+rewrite /is_won !bit_logand2 // -!negb_exists.
+case: existsP => /= [[i /and4P[H1 H2 H3 H4]]|Hh].
+  apply/sym_equal/existsP.
+  exists i; apply/existsP; exists horizontal.
+  by rewrite inE eqxx H1 H2 H3 H4.
+case: existsP => /= [[i /and4P[H1 H2 H3 H4]]|Hv].
+  apply/sym_equal/existsP.
+  exists i; apply/existsP; exists vertical.
+  by rewrite !inE eqxx andTb H1 H2 H3 H4.
+case: existsP => /= [[i /and4P[H1 H2 H3 H4]]|Hur].
+  apply/sym_equal/existsP.
+  exists i; apply/existsP; exists up_right.
+  by rewrite !inE eqxx andTb H1 H2 H3 H4.
+case: existsP => /= [[i /and4P[H1 H2 H3 H4]]|Hul].
+  apply/sym_equal/existsP.
+  exists i; apply/existsP; exists up_left.
+  by rewrite !inE eqxx andTb H1 H2 H3 H4.
+apply/sym_equal/idP => /existsP [i /existsP [dir /and5P[]]].
+rewrite !inE; case/or4P => /eqP-> H1 H2 H3 H4.
+- by case: Hh; exists i; rewrite H1 H2 H3 H4.
+- by case: Hv; exists i; rewrite H1 H2 H3 H4.
+- by case: Hul; exists i; rewrite H1 H2 H3 H4.
+by case: Hur; exists i; rewrite H1 H2 H3 H4.
+Qed.
+
+Definition get_column (state : int) (i : int) :=
+  let state1 := if i =? 0 then state else
+     (state >> ((i - 1) * horizontal)) in
+  state1 land full_first_column.
+
+Lemma eqb_eqb (i j : int) : (i =? j) = (i == j).
+Proof.
+case: (_ =P _) => [->|]; case: eqbP; try lia.
+by move=> iEj []; apply: to_Z_inj.
+Qed.
+
+Lemma mul_0_l i : 0 * i = 0.
+Proof.
+apply: to_Z_inj.
+by rewrite mul_spec Z.mul_0_l Z.mod_0_l.
+Qed.
+
+Lemma mul_1_l i : 1 * i = i.
+Proof.
+apply: to_Z_inj.
+rewrite mul_spec Z.mul_1_l Z.mod_small //; apply: to_Z_bounded.
+Qed.
+
+Lemma add_0_l i : 0 + i = i.
+Proof.
+apply: to_Z_inj.
+by rewrite add_spec Z.add_0_l Z.mod_small //; apply: to_Z_bounded.
+Qed.
+
+Lemma bit_get_colum s i j : 
+  i <=? width -> j <=? height ->
+  bit (get_column s i) j = bit s ((i != 0) * (i - 1) * horizontal + j).
+Proof.
+have iB := to_Z_bounded i.
+have jB := to_Z_bounded j.
+case: lebP => // iLw.
+case: lebP => // jLh _ _.
+have hEh : φ (horizontal) = (φ (height) + 1)%Z by [].
+rewrite /get_column eqb_eqb.
+case: (_ =P 0) => [_ | /eqP iD0].
+  rewrite mul_0_l add_0_l land_spec full_first_colum_spec andbC.
+  by case: (ltbP j) => //; lia.
+have iP : (0 < φ (i))%Z.
+  rewrite -eqb_eqb in iD0; case: eqbP iD0 => //.
+  by rewrite -[to_Z 0]/0%Z; lia.
+rewrite land_spec full_first_colum_spec andbC mul_1_l.
+case: (ltbP j) => [_|]; last by lia.
+rewrite andTb bit_lsr; case: lebP => //; try lia.
+rewrite !(sub_spec, add_spec, mul_spec) -[to_Z 1]/1%Z.
+rewrite [((_ - _) mod wB)%Z]Z.mod_small; last by lia.
+rewrite [((_ * _) mod wB)%Z]Z.mod_small; last first.
+  split; try nia.
+  suff : (φ (width) * φ (horizontal) < wB)%Z by nia.
+  by [].
+rewrite Z.mod_small; first by nia.
+suff : (φ (width) * φ (horizontal) < wB)%Z by nia.
+by [].
+Qed.
+
+(** (one)^*(zero)^+ *)
+Definition opzs (i : int) :=
+  [exists j : int, (j <? digits) && [forall k : int,  bit i k == (k <? j)]].
+
+Lemma opzsE i : opzs i = [exists j, (j <? digits) && (i == decr (one << j))].
+Proof.
+apply/existsP/existsP => [[k /andP[kLd /forallP Hb]]|[k /andP[kLd /eqP iEd]]].
+  exists k; rewrite kLd.
+  apply/eqP/bit_ext => j.
+  by rewrite bit_decr; have := eqP (Hb j).
+exists k; rewrite kLd; apply/forallP => j.
+by rewrite iEd bit_decr.
+Qed.
+
+Lemma is_zero_0 : is_zero 0.
+Proof. by apply/is_zero_spec. Qed.
+
+Lemma bit_le i j : (i <? (one << j)) -> bit i j = false.
+Proof.
+have iB := to_Z_bounded i.
+case: ltbP => //.
+rewrite lsl_spec Z.mul_1_l.
+case: (Z.le_decidable (φ (digits)) (φ (j))) => jLd; last first.
+  rewrite Z.mod_small; last first.
+    split; try lia.
+    apply: Z.pow_lt_mono_r; try lia.
+    by rewrite -[IntDef.Z.of_nat size]/(φ (digits)); lia.
+  move=> iLj; rewrite /bit.
+  suff -> : (i >> j) = 0 by rewrite lsl0 is_zero_0.
+  by apply: to_Z_inj; rewrite lsr_spec to_Z_0 Z.div_small; lia.
+rewrite Znumtheory.Zdivide_mod; try lia.
+exists (2 ^ (φ (j) -  φ (digits)))%Z.
+rewrite -Z.pow_add_r; try lia.
+rewrite -[IntDef.Z.of_nat size]/(φ (digits)).
+by congr (_ ^ _)%Z; lia.
+Qed.
+
+Lemma land_power2 i k :
+  k <? digits -> i land (decr (one << k)) = i mod (one << k).
+Proof.
+have iB := to_Z_bounded i.
+have kB := to_Z_bounded k.
+case: ltbP => // kLd _.
+apply: bit_ext => j.
+have jB := to_Z_bounded j.
+rewrite land_spec bit_decr; last by case: ltbP.
+case: ltbP => [jLk|kLj]; rewrite ?(andbT, andbF); last first.
+  have kLj' : (φ (k) <= φ (j))%Z by lia.
+  case: (Z.le_decidable (φ (digits)) (φ (j))) => jLd.
+    by rewrite bit_M //; apply/lebP.
+  apply/sym_equal/bit_le.
+  apply/ltbP.
+  rewrite mod_spec !lsl_spec !Z.mul_1_l.
+  rewrite !(Z.mod_small _ wB); last first.
+  - split; try lia.
+    apply: Z.pow_lt_mono_r; try lia.
+    by rewrite -[IntDef.Z.of_nat size]/(φ (digits)); lia.
+  - split; try lia.
+    apply: Z.pow_lt_mono_r; try lia.
+    by rewrite -[IntDef.Z.of_nat size]/(φ (digits)); lia.
+  apply: Z.lt_le_trans (_ : (_ < 2 ^ φ (k))%Z) _.
+    by have := Z.mod_pos_bound (φ (i)) (2 ^ (φ (k))); lia.
+  by apply: Z.pow_le_mono_r; lia.
+rewrite /bit.
+congr (~~ is_zero _).
+apply: to_Z_inj.
+rewrite !(lsr_spec, lsl_spec, mod_spec) ?Z.mul_1_l.
+rewrite !(Z.mod_small (2 ^ φ (k)) wB); last first.
+  split; try lia.
+  apply: Z.pow_lt_mono_r; try lia.
+  by rewrite -[IntDef.Z.of_nat size]/(φ (digits)); lia.
+rewrite {1}(Z_div_mod_eq_full (φ (i)) (2 ^ φ (k))).
+have {1}-> : φ (k) = (φ (j) + ((φ (k) - φ (j) - 1) + 1))%Z by lia.
+rewrite Z.pow_add_r; try lia.
+rewrite -[((2 ^ φ (j) * _) * _)%Z]Z.mul_assoc [(2 ^ φ (j) * _)%Z]Z.mul_comm.
+rewrite Z.div_add_l; try lia.
+rewrite Z.mul_add_distr_r.
+rewrite -Zplus_mod_idemp_l.
+set u := ((_ * _ ) mod wB)%Z.
+suff -> : u = 0%Z by rewrite Z.add_0_l; lia.
+rewrite /u Z.pow_add_r; try lia.
+set v := (2 ^ (_ - _))%Z; set w := (_ / _)%Z; set t := (2 ^ (to_Z (_ - _)))%Z.
+have -> : (v * 2 ^ 1 * w * t = v * w * (2 ^ 1 * t))%Z by lia.
+suff -> : (2 ^ 1 * t = wB)%Z by rewrite Z_mod_mult.
+rewrite -Z.pow_add_r; try lia.
+  by congr (2 ^ _)%Z.
+rewrite /to_Z /=; lia.
+Qed.
+
+Definition get_border (wstate bstate : int) :=
+  bottom + (wstate lor bstate).
+
+(* Perform a move *)
+Definition  make_move move state := move lor state.
+
+(* Get the log 2 of a number *)
+Definition get_log2 (v : int) : int :=
+   62 - head0 v.
+
+(* List of possible moves, no move = draw *)
+Inductive moves := EmptyMove | Move (m : int) (v : int) (l : moves).
+
+(* Moves are ordered by their values *)
+Fixpoint insert_fmove m (v : int) l := 
+match l with 
+| EmptyMove => Move m v EmptyMove
+| Move m1 v1 l1 => 
+  match v ?= v1 with
+  |Lt => Move m1 v1 (insert_fmove m v l1)
+  | _ => Move m v l
+  end
+end.
+
+Inductive fmove := 
+ | Win
+ | Draw
+ | Forced (_ : int)
+ | Moves (_: moves).
+
+Definition make_moves l :=
+  match l with EmptyMove => Draw | _ => Moves l end.
+
+Section FindMoves.
+
+Variables (wstate bstate border: int).
+
+Fixpoint make_colums i column :=
+  match i with
+      O => nil 
+  | S i => column :: (make_colums i (column << horizontal))
+  end.
+
+Definition columns := Eval compute in make_colums nwidth first_column.
+
+(* Check for a direct win after a threat *)
+Fixpoint fmt columns res :=
+  match columns with 
+  | nil => res
+  | column :: columns =>
+      let move := border land column in
+      if is_zero move then fmt columns res
+      else
+      if is_won (make_move move wstate) then Win
+      else fmt columns res
+  end.
+
+Fixpoint fms columns res :=
+  match columns with 
+  | nil => make_moves res
+  | column :: columns =>
+      let move := border land column in
+      if is_zero move then fms columns res
+      else
+      if is_won (make_move move wstate) then Win
+      else
+      if is_won (make_move move bstate) then 
+        fmt columns (Forced move)
+      else
+        let v := (values.[get_log2 move]) in
+        fms columns (insert_fmove move v res)
+   end.
+
+Lemma fmsE columns res :
+fms columns res =
+  match columns with 
+  | nil => make_moves res
+  | column :: columns =>
+      let move := border land column in
+      if is_zero move then fms columns res
+      else
+      if is_won (make_move move wstate) then Win
+      else
+      if is_won (make_move move bstate) then 
+        fmt columns (Forced move)
+      else
+        let v := (values.[get_log2 move]) in
+        fms columns (insert_fmove move v res)
+   end.
+Proof.
+by case: columns.
+Qed.
+
+End FindMoves.
+
+(* Find possible moves *)
+Definition find_moves wstate bstate :=
+  let border := get_border wstate bstate in
+  fms wstate bstate border columns EmptyMove.
+
+(* Auxillary parsing function from string to states *)
+Fixpoint parsei s i j wstate bstate (turn : bool) :=
+  match
+    match width ?= j with 
+    |Eq => 
+       match i ?= 0 with Eq => None | _ => Some (i-1,0) end
+    | _ => Some (i,j) end
+  with None => (wstate,bstate,turn)
+  | Some (i,j) =>
+    match s with
+    | EmptyString => (wstate,bstate,turn)
+    | String "X"%char s1 =>
+       let move := one << (j * horizontal + i) in 
+       parsei s1 i (j + 1) (make_move wstate move) bstate (negb turn)
+    | String "O"%char s1 =>
+       let move := one << (j * horizontal + i) in 
+       parsei s1 i (j + 1) wstate (make_move bstate move) (negb turn)
+    | String "_"%char s1 => 
+       parsei s1 i (j + 1) wstate bstate turn
+    | String _ s1 => parsei s1 i j wstate bstate turn
+    end
+  end.
+
+(* Parsing function from string to states *)
+Definition parse_string s :=
+  parsei s height width zero zero true.
+
+(* Newline String *)
+Definition nl := String "013" EmptyString.
+
+(* Auxillary function that turns states into into a string *)
+Fixpoint to_stringi m i j wstate bstate :=
+  match m with O => ""%string | (S m1) => 
+  match
+    match width ?= j with 
+    |Eq => 
+       match i ?= 0 with Eq => None | _ => Some (i-1,0,nl) end
+    | _ => Some (i,j,""%string) end
+  with
+  | None => nl
+  | Some (i,j,ts) =>
+    (ts ++
+   (let move := one << (j * horizontal + i) in 
+    if is_nzero (move land wstate) then "X"%string ++ (to_stringi m1 i (j + 1) wstate bstate) 
+    else if is_nzero (move land bstate) then "O"%string ++ (to_stringi m1 i (j + 1) wstate bstate) 
+    else "_"%string ++ (to_stringi m1 i (j + 1) wstate bstate)))%string
+  end
+  end.
+
+(* Turn states into a string *)
+Definition to_string wstate bstate :=
+ (to_stringi (nheight * nwidth) height width wstate bstate)%string.
+
+(* Turn the score in a string *)
+Definition string_of_score (score : int) :=
+  if eqb score unknown then "UNKNOWN"%string else
+  if eqb score loss then "LOSS"%string else
+  if eqb score draw then "DRAW"%string else
+  if eqb score win then "WIN"%string else
+  if eqb score drawwin then "DRAWWIN"%string else
+  if eqb score lossdraw then "LOSSDRAW"%string else
+  "????"%string.
+
+(* Reverse the valuation *)
+Definition rev_val value := losswin - value.
+
+Fixpoint sym_code i sres res :=
+  match i with 
+  | O => sres
+  | S i =>
+      let sres :=  (sres << horizontal) lor
+                       (res land full_first_column) in
+      let res := res >> horizontal in
+      sym_code i sres res
+  end.
+    
+(* Get the unique code of a position *)
+Definition get_code wstate bstate turn height :=
+  let res := (match turn with true => wstate | false => bstate end) lor
+        (get_border wstate bstate) in
+  if height <=? sym_level
+  then
+     let sres := sym_code nwidth zero res in
+     min sres res
+  else res.
+
+(* Put an element in the hash-table
+    The layout of the two-entry hash-table
+      at key : high bits = work first entry, low bits = lock first entry
+      at key + 1 : high bits = score first entry then score second entry
+                   low bits = lock second entry
+ *)
+
+Definition hput wstate bstate turn work score hash_table height :=
+   if (score land 1) =? 0 then hash_table
+   else
+   let code := get_code wstate bstate turn height in
+   let fkey := code mod hprime in
+   let key := 2 * (fkey >> lhash) in
+   let r :=  fkey land mhash in
+   let lock := (code >> slocksize) in
+   let ht := (hash_table.[r]) in
+   let val1 := (ht.[key]) in
+   let val2 := (ht.[key + 1]) in
+   if orb ((val1 land lockmask) =? lock) ((val1 >> locksize) <=? work) then
+       let ht := (ht.[key <- (work << locksize) lor lock]) in
+       let ht := (ht.[key + 1 <- 
+                   ((score << scorelocksize) lor (val2 land scorelockmask))]) in
+        (hash_table.[r <- ht])
+   else
+      let ht := (ht.[key + 1 <-
+        ((((val2 >> scorelocksize) << scoresize) lor score) << locksize)
+              lor lock]) in
+        (hash_table.[r <- ht]).
+
+(* Get an element in the hash-table *)
+Definition hget (wstate bstate : int) (turn : bool) 
+         (hash_table : array (array int)) height := 
+   let code := get_code wstate bstate turn height in
+   let fkey := code mod hprime in
+   let key := 2 * (fkey >> lhash) in
+   let r :=  fkey land mhash in
+   let lock := (code >> slocksize) in
+   let ht := (hash_table.[r]) in
+   let val1 := (ht.[key]) in
+   let val2 := (ht.[key + 1]) in
+   if ((val1 land lockmask) =? lock) then
+       val2 >> scorelocksize
+   else if ((val2 land lockmask) =? lock) then
+       (val2 >> locksize) land scoremask
+   else unknown.
+
+Definition is_nempty_move m :=
+  match m with EmptyMove => false | Move _ _ _ => true end.
+
+(* Process result *)
+Inductive pres := PRes (s : int) (v : int) (t : array (array int)).
+
+Section Process.
+
+Variables (wstate bstate : int) (turn : bool) (beta : int) (lvisited : int) 
+          (height hscore :  int)
+          (alpha_beta : int -> int -> bool -> int -> int -> int -> 
+                         array (array int) -> pres).
+Fixpoint process ms alpha score visited hash_table :=
+  match ms with
+  | EmptyMove =>
+      let score := if (score =? losswin - hscore) then draw else score in
+      let work := get_log2 (sub visited lvisited) in
+      let hash_table := hput wstate bstate turn work score hash_table height in
+      PRes score (incr visited) hash_table
+  | Move move _ ms1 =>
+    let (nscore,visited,hash_table) := 
+      alpha_beta bstate (make_move move wstate) (negb turn)
+           (rev_val beta) (rev_val alpha) visited hash_table in
+    let nscore := rev_val nscore in
+    if nscore <=? score then process ms1 alpha score visited hash_table 
+    else
+    let score := nscore in
+    if score <=? alpha then process ms1 alpha score visited hash_table                 
+    else
+    let alpha := score in
+    if alpha <? beta  then process ms1 alpha score visited hash_table 
+    else
+      let score :=
+        if (andb (score =? draw) (is_nempty_move ms1)) then drawwin 
+        else score in
+      let score := if (score =? losswin - hscore) then draw else score in
+      let work := get_log2 (sub visited  lvisited) in
+      let hash_table := hput wstate bstate turn work score hash_table height in
+      PRes score (incr visited) hash_table
+    end.
+
+End Process.
+
+(* alpha-beta result *)
+Inductive ares := ARes (a : int) (b : int) (c : bool).
+
+Section Alpha.
+
+(* alpha beta pruning search *)
+Fixpoint alpha_beta nstruct height wstate bstate turn alpha beta 
+                    visited hash_table :=
+  let hscore := hget wstate bstate turn hash_table height in
+  let (alpha,beta,flag) :=
+    (if (hscore =? unknown) then ARes alpha beta false else
+    if negb ((hscore land 1) =? 0) then ARes alpha beta true else
+    if (hscore =? drawwin) then
+      if (beta =? draw) then ARes alpha beta true else ARes draw beta false
+    else
+      if (alpha =? draw) then ARes alpha beta true 
+      else ARes alpha draw false) in
+  if flag then PRes hscore visited hash_table else
+  match find_moves wstate bstate with
+  | Win => PRes win visited hash_table
+  | Draw => PRes draw visited hash_table
+  | Forced move =>
+      match nstruct with 
+     | 0%nat => PRes unknown visited hash_table
+     | S nstruct =>
+      let (score,visited,hash_table) := 
+        alpha_beta nstruct (height + 1) bstate (make_move move wstate) 
+                   (negb turn) (rev_val beta) (rev_val alpha) 
+                    visited hash_table : pres in
+      PRes (rev_val score) visited hash_table 
+     end
+  | Moves ms =>
+     match nstruct with 
+     | 0%nat => PRes unknown visited hash_table
+     | S nstruct =>
+     process wstate bstate turn beta visited height hscore 
+            (alpha_beta nstruct (height + 1))
+             ms alpha loss visited hash_table
+     end
+  end.
+
+Lemma alpha_betaE nstruct height wstate bstate turn alpha beta 
+                    visited hash_table  :
+ alpha_beta nstruct height wstate bstate turn alpha beta 
+                    visited hash_table =
+  let hscore := hget wstate bstate turn hash_table height in
+  let (alpha,beta,flag) :=
+    (if (hscore =? unknown) then ARes alpha beta false else
+    if negb ((hscore land 1) =? 0) then ARes alpha beta true else
+    if (hscore =? drawwin) then
+      if (beta =? draw) then ARes alpha beta true else ARes draw beta false
+    else
+      if (alpha =? draw) then ARes alpha beta true 
+      else ARes alpha draw false) in
+  if flag then PRes hscore visited hash_table else
+  match find_moves wstate bstate with
+  | Win => PRes win visited hash_table
+  | Draw => PRes draw visited hash_table
+  | Forced move =>
+      match nstruct with 
+     | 0%nat => PRes unknown visited hash_table
+     | S nstruct =>
+      let (score,visited,hash_table) := 
+        alpha_beta nstruct (height + 1) bstate (make_move move wstate) 
+                   (negb turn) (rev_val beta) (rev_val alpha) 
+                    visited hash_table : pres in
+      PRes (rev_val score) visited hash_table 
+     end
+  | Moves ms =>
+     match nstruct with 
+     | 0%nat => PRes unknown visited hash_table
+     | S nstruct =>
+     process wstate bstate turn beta visited height hscore 
+            (alpha_beta nstruct (height + 1))
+             ms alpha loss visited hash_table
+     end
+  end.
+Proof. by case: nstruct. Qed.
+
+Definition eval_position s :=
+   match parse_string s with
+   (wstate,bstate,turn) =>
+   let (wstate,bstate) := if turn then (wstate,bstate) else (bstate,wstate) in
+   let (score, _, _) :=
+     alpha_beta (1 + nheight * nwidth)%nat 0 wstate bstate turn loss win zero
+                (make_hash tt) in
+   score
+   end.
+
+End Alpha.
+
+Definition ex1 := (
+                 "___O___"
+              ++ "___X___"
+              ++ "___O___"
+              ++ "___X___"
+              ++ "__OO___"
+              ++ "__XX___")%string.
+
+
+Definition ex2 := (
+                 "___X___"
+              ++ "__OX___"
+              ++ "__XO___"
+              ++ "__OX___"
+              ++ "__XO___"
+              ++ "__OX__O")%string.
+
+
+Definition ex3 := (
+                 "___O___"
+              ++ "___X___" 
+              ++ "___O___"
+              ++ "___X___"
+              ++ "___O___"
+              ++ "XO_X___")%string.
+
+Definition ex4 := ("______" ++ "______" ++ "______" ++
+                   "______" ++ "______" ++ "______" ++ "______")%string.
+
+Time Eval native_compute in string_of_score (eval_position ex1).
+Time Eval native_compute in string_of_score (eval_position ex2).
+Time Eval native_compute in string_of_score (eval_position ex3).
+Time Eval native_compute in string_of_score (eval_position ex4).
+
+
